examples/ProcDecInv.v
@@ -1,0 +1,115 @@
+Require Import Bool String List.
+Require Import Lib.CommonTactics Lib.ilist Lib.Word.
+Require Import Lib.Struct Lib.StringBound Lib.FMap Lib.StringEq.
+Require Import Lts.Syntax Lts.Semantics Lts.Equiv Lts.Refinement Lts.Renaming Lts.Wf.
+Require Import Lts.Renaming Lts.Specialize Lts.Inline Lts.InlineFacts_2 Lts.Decomposition.
+Require Import Ex.SC Ex.Fifo Ex.MemAtomic Ex.ProcDec.
+Require Import Eqdep.
+
+Set Implicit Arguments.
+
+Ltac kgetv k v m t f :=
+  destruct (M.find k m) as [[[kind|] v]|]; [|exact f|exact f];
+  destruct (decKind kind t); [subst|exact f].
+
+Ltac kexistv k v m t :=
+  refine (exists v: fullType type (SyntaxKind t),
+             M.find k m = Some (existT _ _ v) /\ _).
+
+Section Invariants.
+  Variables addrSize fifoSize valSize rfIdx: nat.
+
+  Variable dec: DecT 2 addrSize valSize rfIdx.
+  Variable exec: ExecT 2 addrSize valSize rfIdx.
+
+  Definition procDec_inv_0 (o: RegsT): Prop.
+  Proof.
+    kexistv "pc"%string pcv o (Bit addrSize).
+    kexistv "rf"%string rfv o (Vector (Bit valSize) rfIdx).
+    kexistv "stall"%string stallv o Bool.
+    kexistv "Ins.empty"%string iev o Bool.
+    kexistv "Ins.full"%string ifv o Bool.
+    kexistv "Ins.enqP"%string ienqpv o (Bit fifoSize).
+    kexistv "Ins.deqP"%string ideqpv o (Bit fifoSize).
+    kexistv "Ins.elt"%string ieltv o (Vector (memAtomK addrSize valSize) fifoSize).
+    kexistv "Outs.empty"%string oev o Bool.
+    kexistv "Outs.full"%string ofv o Bool.
+    kexistv "Outs.enqP"%string oenqpv o (Bit fifoSize).
+    kexistv "Outs.deqP"%string odeqpv o (Bit fifoSize).
+    kexistv "Outs.elt"%string oeltv o (Vector (memAtomK addrSize valSize) fifoSize).
+    exact True.
+  Defined.
+
+  Definition xor3 (b1 b2 b3: bool) :=
+    (b1 && (negb b2) && (negb b3))
+    || ((negb b1) && b2 && (negb b3))
+    || ((negb b1) && (negb b2) && b3).
+  
+  Definition procDec_inv_1 (o: RegsT): Prop.
+  Proof.
+    kexistv "stall"%string stallv o Bool.
+    kexistv "Ins.empty"%string iev o Bool.
+    kexistv "Outs.empty"%string oev o Bool.
+    exact (xor3 (negb v) (negb v0) (negb v1) = true).
+  Defined.
+
+  Definition pdec := pdecf fifoSize dec exec.
+  Hint Unfold pdec: ModuleDefs. (* for kinline_compute *)
+
+  Definition pdecInl: Modules * bool.
+  Proof.
+    remember (inlineF pdec) as inlined.
+    kinline_compute_in Heqinlined.
+    match goal with
+    | [H: inlined = ?m |- _] =>
+      exact m
+    end.
+  Defined.
+
+  Lemma pdecInl_equal: pdecInl = inlineF pdec.
+  Proof.
+    admit.
+    (* kinline_compute. *)
+    (* reflexivity. *)
+  Qed.
+
+  Lemma procDec_inv_0_ok':
+    forall init n ll,
+      init = initRegs (getRegInits (fst pdecInl)) ->
+      Multistep (fst pdecInl) init n ll ->
+      procDec_inv_0 n.
+  Proof.
+    admit.
+    (* induction 2. *)
+
+    (* - repeat subst. *)
+    (*   simpl; unfold procDec_inv_0. *)
+      
+    (*   repeat ( *)
+    (*       try eexists; *)
+    (*       repeat rewrite M.find_add_2 by discriminate; *)
+    (*       repeat rewrite M.find_add_1 by reflexivity). *)
+
+    (* - specialize (IHMultistep H); clear -IHMultistep HStep. *)
+    (*   admit. *)
+  Qed.
+
+  Lemma procDec_inv_0_ok:
+    forall o,
+      reachable o (fst pdecInl) ->
+      procDec_inv_0 o.
+  Proof.
+    intros; inv H; inv H0.
+    eapply procDec_inv_0_ok'; eauto.
+  Qed.
+
+  Lemma procDec_inv_1_ok:
+    forall o,
+      reachable o (fst pdecInl) ->
+      procDec_inv_1 o.
+  Proof.
+    admit.
+  Qed.
+
+End Invariants.
+
